src/SlowPrimeSynthesisExamples.v
@@ -85,11 +85,11 @@ Module debugging_solinas_reduction.
       let prod1 := Saturated.Associational.sat_mul base (skipn 3 p_a) (firstn 2 (skipn 1 p_a)) in
       (* first carry chain *)
       let carry1_a := prod0 ++ prod1 in
-      let carry1_rows := Saturated.Rows.from_associational weight 7 carry1_a in
-      let carry1 := Saturated.Rows.flatten weight 7 carry1_rows in
+      let carry1_rows := Saturated.Rows.from_associational weight 8 carry1_a in
+      let carry1 := Saturated.Rows.flatten weight 8 carry1_rows in
       (* a1 * [a2], second carry chain *)
       let prod2 := Saturated.Associational.sat_mul base (firstn 1 (skipn 1 p_a)) (firstn 1 (skipn 2 p_a)) in
-      let carry2_rows := Saturated.Rows.from_associational weight 7 prod2 in
+      let carry2_rows := Saturated.Rows.from_associational weight 8 prod2 in
       let carry2 := Saturated.Rows.flatten' weight carry1 carry2_rows in
       (* doubling, third carry chain *)
       let carry2 := (fst carry2) ++ [snd carry2] in
@@ -97,13 +97,32 @@ Module debugging_solinas_reduction.
       (* squaring, fourth carry chain *)
       let square_a := sqr_indiv base p_a in
       let square_rows := Saturated.Rows.from_associational weight 8 square_a in
-      let square := Saturated.Rows.flatten weight 8 square_rows in
+      let square := Saturated.Rows.flatten' weight double square_rows in
       fst square.
 
     Definition squaremod base s c (n : Z) (p : list Z) :=
       let sqr := square_no_reduce base p in
       let r := reduce_full' base s c 4 sqr in
       r.
+
+    Print Z.add_with_get_carry.
+    Print Z.add_with_carry.
+    Print Z.get_carry.
+
+    Definition reduce3 base s c n (p : list Z) :=
+      let bound := (0, 2^machine_wordsize-1) in
+      let bounds := (repeat bound n) ++ [(0, 1)] in
+      let s' := fst (Saturated.Rows.adjust_s weight (S (S n)) s) in
+      let coef_a := Saturated.Associational.sat_mul_const base [(1, s'/s)] c in
+      let coef := Associational.eval coef_a in
+      dlet_nd hi := Z.zselect (nth_default 0 p n) 0 coef in
+          let lo := Z.add_get_carry machine_wordsize hi (nth_default 0 p 0) in
+          if (is_bounded_by bounds p) then
+            [fst lo] ++ (skipn 1 (firstn n p))
+          else
+            let hi' := coef * (nth_default 0 p n) in
+            add_to_nth 0 hi' (firstn n p).
+
 
   End __.
 
@@ -120,6 +139,9 @@ Module debugging_solinas_reduction.
     Let p := [2^64-1; 2^64-1; 2^64-1; 2^64-1].
     Compute (square_no_reduce base p).
     Compute (mul_no_reduce base 4 p p).
+    Let p' := [100; 200; 300; 400].
+    Compute (square_no_reduce base p').
+    Compute (mul_no_reduce base 4 p' p').
 
     Let bound := Some r[0 ~> (2^machine_wordsize - 1)]%zrange.
     Let bound' := Some r[0 ~> (2^machine_wordsize +39)]%zrange.
@@ -150,186 +172,14 @@ Module debugging_solinas_reduction.
             possible_values
             machine_wordsize
             ltac:(let n := (eval cbv in n) in
-                  let r := Reify (squaremod base s c n) in
+                  let r := Reify (square_no_reduce base) in
                   exact r)
                    (fun _ _ => [])
                    (Some (repeat bound (4)), tt)
-                   (Some (repeat bound (4)))
+                   (Some (repeat bound (8)))
                    (None, tt)
                    (None)
            : Pipeline.ErrorT _).
-
-(*
-"Success (""/*
- * Input Bounds:
- *   arg1: [[0x0 ~> 0xffffffffffffffff], [0x0 ~> 0xffffffffffffffff], [0x0 ~> 0xffffffffffffffff], [0x0 ~> 0xffffffffffffffff]]
- * Output Bounds:
- *   out1: [[0x0 ~> 0xffffffffffffffff], [0x0 ~> 0xffffffffffffffff], [0x0 ~> 0xffffffffffffffff], [0x0 ~> 0xffffffffffffffff]]
- */
-void mul(uint64_t out1[4], const uint64_t arg1[4]) {
-  uint64_t x1;
-  uint64_t x2;
-  uint64_t x3;
-  uint64_t x4;
-  uint64_t x5;
-  uint64_t x6;
-  uint64_t x7;
-  uint64_t x8;
-  uint64_t x9;
-  uint64_t x10;
-  uint64_t x11;
-  fiatuint1 x12;
-  uint64_t x13;
-  fiatuint1 x14;
-  uint64_t x15;
-  fiatuint1 x16;
-  uint64_t x17;
-  fiatuint1 x18;
-  uint64_t x19;
-  uint64_t x20;
-  uint64_t x21;
-  uint64_t x22;
-  fiatuint1 x23;
-  uint64_t x24;
-  fiatuint1 x25;
-  uint64_t x26;
-  fiatuint1 x27;
-  uint64_t x28;
-  fiatuint1 x29;
-  uint64_t x30;
-  fiatuint1 x31;
-  uint64_t x32;
-  fiatuint1 x33;
-  uint64_t x34;
-  fiatuint1 x35;
-  uint64_t x36;
-  fiatuint1 x37;
-  uint64_t x38;
-  fiatuint1 x39;
-  uint64_t x40;
-  fiatuint1 x41;
-  uint64_t x42;
-  uint64_t x43;
-  uint64_t x44;
-  uint64_t x45;
-  uint64_t x46;
-  uint64_t x47;
-  uint64_t x48;
-  uint64_t x49;
-  uint64_t x50;
-  uint64_t x51;
-  fiatuint1 x52;
-  uint64_t x53;
-  fiatuint1 x54;
-  uint64_t x55;
-  fiatuint1 x56;
-  uint64_t x57;
-  fiatuint1 x58;
-  uint64_t x59;
-  fiatuint1 x60;
-  uint64_t x61;
-  fiatuint1 x62;
-  uint64_t x63;
-  fiatuint1 x64;
-  uint64_t x65;
-  uint64_t x66;
-  uint64_t x67;
-  uint64_t x68;
-  uint64_t x69;
-  uint64_t x70;
-  uint64_t x71;
-  uint64_t x72;
-  uint64_t x73;
-  fiatuint1 x74;
-  uint64_t x75;
-  fiatuint1 x76;
-  uint64_t x77;
-  fiatuint1 x78;
-  uint64_t x79;
-  uint64_t x80;
-  fiatuint1 x81;
-  uint64_t x82;
-  fiatuint1 x83;
-  uint64_t x84;
-  fiatuint1 x85;
-  uint64_t x86;
-  fiatuint1 x87;
-  uint64_t x88;
-  uint64_t x89;
-  uint64_t x90;
-  uint64_t x91;
-  fiatuint1 x92;
-  uint64_t x93;
-  fiatuint1 x94;
-  uint64_t x95;
-  fiatuint1 x96;
-  uint64_t x97;
-  fiatuint1 x98;
-  uint64_t x99;
-  fiatuint128 x100;
-  uint64_t x101;
-  fiatmulx_u64(&x1, &x2, (arg1[0]), (arg1[3]));
-  fiatmulx_u64(&x3, &x4, (arg1[0]), (arg1[2]));
-  fiatmulx_u64(&x5, &x6, (arg1[0]), (arg1[1]));
-  fiatmulx_u64(&x7, &x8, (arg1[3]), (arg1[2]));
-  fiatmulx_u64(&x9, &x10, (arg1[3]), (arg1[1]));
-  fiataddcarryx_u64(&x11, &x12, 0x0, x6, x3);
-  fiataddcarryx_u64(&x13, &x14, x12, x4, x1);
-  fiataddcarryx_u64(&x15, &x16, x14, x2, x9);
-  fiataddcarryx_u64(&x17, &x18, x16, x10, x7);
-  x19 = (x18 + x8);
-  fiatmulx_u64(&x20, &x21, (arg1[1]), (arg1[2]));
-  fiataddcarryx_u64(&x22, &x23, 0x0, x13, x20);
-  fiataddcarryx_u64(&x24, &x25, x23, x15, x21);
-  fiataddcarryx_u64(&x26, &x27, x25, x17, 0x0);
-  fiataddcarryx_u64(&x28, &x29, x27, x19, 0x0);
-  fiataddcarryx_u64(&x30, &x31, 0x0, x5, x5);
-  fiataddcarryx_u64(&x32, &x33, x31, x11, x11);
-  fiataddcarryx_u64(&x34, &x35, x33, x22, x22);
-  fiataddcarryx_u64(&x36, &x37, x35, x24, x24);
-  fiataddcarryx_u64(&x38, &x39, x37, x26, x26);
-  fiataddcarryx_u64(&x40, &x41, x39, x28, x28);
-  x42 = (((uint64_t)x41 + x29) + (uint64_t)x29);
-  fiatmulx_u64(&x43, &x44, (arg1[3]), (arg1[3]));
-  fiatmulx_u64(&x45, &x46, (arg1[2]), (arg1[2]));
-  fiatmulx_u64(&x47, &x48, (arg1[1]), (arg1[1]));
-  fiatmulx_u64(&x49, &x50, (arg1[0]), (arg1[0]));
-  fiataddcarryx_u64(&x51, &x52, 0x0, x50, x30);
-  fiataddcarryx_u64(&x53, &x54, x52, x47, x32);
-  fiataddcarryx_u64(&x55, &x56, x54, x48, x34);
-  fiataddcarryx_u64(&x57, &x58, x56, x45, x36);
-  fiataddcarryx_u64(&x59, &x60, x58, x46, x38);
-  fiataddcarryx_u64(&x61, &x62, x60, x43, x40);
-  fiataddcarryx_u64(&x63, &x64, x62, x44, x42);
-  fiatmulx_u64(&x65, &x66, UINT8_C(0x26), x63);
-  fiatmulx_u64(&x67, &x68, UINT8_C(0x26), x61);
-  fiatmulx_u64(&x69, &x70, UINT8_C(0x26), x59);
-  fiatmulx_u64(&x71, &x72, UINT8_C(0x26), x57);
-  fiataddcarryx_u64(&x73, &x74, 0x0, x51, x69);
-  fiataddcarryx_u64(&x75, &x76, x74, x53, x67);
-  fiataddcarryx_u64(&x77, &x78, x76, x55, x65);
-  x79 = (x78 + x66);
-  fiataddcarryx_u64(&x80, &x81, 0x0, x49, x71);
-  fiataddcarryx_u64(&x82, &x83, x81, x73, x72);
-  fiataddcarryx_u64(&x84, &x85, x83, x75, x70);
-  fiataddcarryx_u64(&x86, &x87, x85, x77, x68);
-  x88 = (x87 + x79);
-  fiatmulx_u64(&x89, &x90, UINT8_C(0x26), x88);
-  fiataddcarryx_u64(&x91, &x92, 0x0, x80, x89);
-  fiataddcarryx_u64(&x93, &x94, x92, x82, 0x0);
-  fiataddcarryx_u64(&x95, &x96, x94, x84, 0x0);
-  fiataddcarryx_u64(&x97, &x98, x96, x86, 0x0);
-  fiatcmovznz_u64(&x99, x98, 0x0, UINT8_C(0x26));
-  x100 = ((fiatuint128)x99 + x91);
-  x101 = (uint64_t)(x100 & UINT64_C(0xffffffffffffffff));
-  out1[0] = x101;
-  out1[1] = x93;
-  out1[2] = x95;
-  out1[3] = x97;
-}"", {| bitwidths_used := [uint128, uint1, uint64] ; addcarryx_lg_splits := [64] ; mulx_lg_splits := [64] ; cmovznz_bitwidths := [uint64] ; value_barrier_bitwidths := [] ; typedefs_used := [] |})"
-     : string
-Finished transaction in 4.494 secs (4.41u,0.066s) (successful)
-*)
 
     Time Compute
          Show.show
@@ -348,226 +198,6 @@ Finished transaction in 4.494 secs (4.41u,0.066s) (successful)
                    (None, (None, tt))
                    (None)
            : Pipeline.ErrorT _).
-(*
-/*
- * Input Bounds:
- *   arg1: [[0x0 ~> 0xffffffffffffffff], [0x0 ~> 0xffffffffffffffff], [0x0 ~> 0xffffffffffffffff], [0x0 ~> 0xffffffffffffffff]]
- *   arg2: [[0x0 ~> 0xffffffffffffffff], [0x0 ~> 0xffffffffffffffff], [0x0 ~> 0xffffffffffffffff], [0x0 ~> 0xffffffffffffffff]]
- * Output Bounds:
- *   out1: None
- */
-void f(uint128 out1[4], const uint64_t arg1[4], const uint64_t arg2[4]) {
-  uint64_t x1;
-  uint64_t x2;
-  uint64_t x3;
-  uint64_t x4;
-  uint64_t x5;
-  uint64_t x6;
-  uint64_t x7;
-  uint64_t x8;
-  uint64_t x9;
-  uint64_t x10;
-  uint64_t x11;
-  uint64_t x12;
-  uint64_t x13;
-  uint64_t x14;
-  uint64_t x15;
-  uint64_t x16;
-  uint64_t x17;
-  uint64_t x18;
-  uint64_t x19;
-  uint64_t x20;
-  uint64_t x21;
-  uint64_t x22;
-  uint64_t x23;
-  uint64_t x24;
-  uint64_t x25;
-  uint64_t x26;
-  uint64_t x27;
-  uint64_t x28;
-  uint64_t x29;
-  uint64_t x30;
-  uint64_t x31;
-  uint64_t x32;
-  uint64_t x33;
-  uint1 x34;
-  uint64_t x35;
-  uint1 x36;
-  uint64_t x37;
-  uint64_t x38;
-  uint1 x39;
-  uint64_t x40;
-  uint1 x41;
-  uint64_t x42;
-  uint1 x43;
-  uint64_t x44;
-  uint64_t x45;
-  uint1 x46;
-  uint64_t x47;
-  uint1 x48;
-  uint64_t x49;
-  uint1 x50;
-  uint64_t x51;
-  uint1 x52;
-  uint64_t x53;
-  uint1 x54;
-  uint64_t x55;
-  uint64_t x56;
-  uint1 x57;
-  uint64_t x58;
-  uint1 x59;
-  uint64_t x60;
-  uint1 x61;
-  uint64_t x62;
-  uint1 x63;
-  uint64_t x64;
-  uint1 x65;
-  uint64_t x66;
-  uint1 x67;
-  uint64_t x68;
-  uint1 x69;
-  uint64_t x70;
-  uint1 x71;
-  uint64_t x72;
-  uint1 x73;
-  uint64_t x74;
-  uint1 x75;
-  uint64_t x76;
-  uint1 x77;
-  uint64_t x78;
-  uint1 x79;
-  uint64_t x80;
-  uint1 x81;
-  uint64_t x82;
-  uint1 x83;
-  uint64_t x84;
-  uint1 x85;
-  uint64_t x86;
-  uint1 x87;
-  uint64_t x88;
-  uint1 x89;
-  uint64_t x90;
-  uint1 x91;
-  uint64_t x92;
-  uint1 x93;
-  uint64_t x94;
-  uint1 x95;
-  uint64_t x96;
-  uint64_t x97;
-  uint64_t x98;
-  uint64_t x99;
-  uint64_t x100;
-  uint64_t x101;
-  uint64_t x102;
-  uint64_t x103;
-  uint64_t x104;
-  uint1 x105;
-  uint64_t x106;
-  uint1 x107;
-  uint64_t x108;
-  uint1 x109;
-  uint8_t x110;
-  uint64_t x111;
-  uint1 x112;
-  uint64_t x113;
-  uint1 x114;
-  uint64_t x115;
-  uint1 x116;
-  uint64_t x117;
-  uint1 x118;
-  uint8_t x119;
-  uint64_t x120;
-  uint64_t x121;
-  uint64_t x122;
-  uint1 x123;
-  uint64_t x124;
-  uint1 x125;
-  uint64_t x126;
-  uint1 x127;
-  uint64_t x128;
-  uint1 x129;
-  uint8_t x130;
-  uint128 x131;
-  mulx_u64(&x1, &x2, (arg1[3]), (arg2[3]));
-  mulx_u64(&x3, &x4, (arg1[3]), (arg2[2]));
-  mulx_u64(&x5, &x6, (arg1[3]), (arg2[1]));
-  mulx_u64(&x7, &x8, (arg1[3]), (arg2[0]));
-  mulx_u64(&x9, &x10, (arg1[2]), (arg2[3]));
-  mulx_u64(&x11, &x12, (arg1[2]), (arg2[2]));
-  mulx_u64(&x13, &x14, (arg1[2]), (arg2[1]));
-  mulx_u64(&x15, &x16, (arg1[2]), (arg2[0]));
-  mulx_u64(&x17, &x18, (arg1[1]), (arg2[3]));
-  mulx_u64(&x19, &x20, (arg1[1]), (arg2[2]));
-  mulx_u64(&x21, &x22, (arg1[1]), (arg2[1]));
-  mulx_u64(&x23, &x24, (arg1[1]), (arg2[0]));
-  mulx_u64(&x25, &x26, (arg1[0]), (arg2[3]));
-  mulx_u64(&x27, &x28, (arg1[0]), (arg2[2]));
-  mulx_u64(&x29, &x30, (arg1[0]), (arg2[1]));
-  mulx_u64(&x31, &x32, (arg1[0]), (arg2[0]));
-  addcarryx_u64(&x33, &x34, 0x0, x28, x7);
-  addcarryx_u64(&x35, &x36, x34, x26, x5);
-  x37 = (x36 + x18);
-  addcarryx_u64(&x38, &x39, 0x0, x33, x13);
-  addcarryx_u64(&x40, &x41, x39, x35, x8);
-  addcarryx_u64(&x42, &x43, x41, x37, 0x0);
-  x44 = (x43 + x10);
-  addcarryx_u64(&x45, &x46, 0x0, x30, x15);
-  addcarryx_u64(&x47, &x48, x46, x38, x16);
-  addcarryx_u64(&x49, &x50, x48, x40, x11);
-  addcarryx_u64(&x51, &x52, x50, x42, x3);
-  addcarryx_u64(&x53, &x54, x52, x44, 0x0);
-  x55 = (x54 + x2);
-  addcarryx_u64(&x56, &x57, 0x0, x45, x21);
-  addcarryx_u64(&x58, &x59, x57, x47, x19);
-  addcarryx_u64(&x60, &x61, x59, x49, x14);
-  addcarryx_u64(&x62, &x63, x61, x51, x6);
-  addcarryx_u64(&x64, &x65, x63, x53, 0x0);
-  addcarryx_u64(&x66, &x67, x65, x55, 0x0);
-  addcarryx_u64(&x68, &x69, 0x0, x32, x23);
-  addcarryx_u64(&x70, &x71, x69, x56, x24);
-  addcarryx_u64(&x72, &x73, x71, x58, x22);
-  addcarryx_u64(&x74, &x75, x73, x60, x17);
-  addcarryx_u64(&x76, &x77, x75, x62, x9);
-  addcarryx_u64(&x78, &x79, x77, x64, x1);
-  addcarryx_u64(&x80, &x81, x79, x66, 0x0);
-  addcarryx_u64(&x82, &x83, 0x0, x68, x29);
-  addcarryx_u64(&x84, &x85, x83, x70, x27);
-  addcarryx_u64(&x86, &x87, x85, x72, x25);
-  addcarryx_u64(&x88, &x89, x87, x74, x20);
-  addcarryx_u64(&x90, &x91, x89, x76, x12);
-  addcarryx_u64(&x92, &x93, x91, x78, x4);
-  addcarryx_u64(&x94, &x95, x93, x80, 0x0);
-  mulx_u64(&x96, &x97, UINT8_C(0x26), x94);
-  mulx_u64(&x98, &x99, UINT8_C(0x26), x92);
-  mulx_u64(&x100, &x101, UINT8_C(0x26), x90);
-  mulx_u64(&x102, &x103, UINT8_C(0x26), x88);
-  addcarryx_u64(&x104, &x105, 0x0, x82, x100);
-  addcarryx_u64(&x106, &x107, x105, x84, x98);
-  addcarryx_u64(&x108, &x109, x107, x86, x96);
-  x110 = (uint8_t)(x109 + (uint8_t)x97);
-  addcarryx_u64(&x111, &x112, 0x0, x31, x102);
-  addcarryx_u64(&x113, &x114, x112, x104, (uint8_t)x103);
-  addcarryx_u64(&x115, &x116, x114, x106, (uint8_t)x101);
-  addcarryx_u64(&x117, &x118, x116, x108, (uint8_t)x99);
-  x119 = (uint8_t)(x118 + x110);
-  mulx_u64(&x120, &x121, UINT8_C(0x26), x119);
-  addcarryx_u64(&x122, &x123, 0x0, x111, (uint16_t)x120);
-  addcarryx_u64(&x124, &x125, x123, x113, 0x0);
-  addcarryx_u64(&x126, &x127, x125, x115, 0x0);
-  addcarryx_u64(&x128, &x129, x127, x117, 0x0);
-  cmovznz_u8(&x130, x129, 0x0, UINT8_C(0x26));
-  x131 = (x130 + (uint128)x122);
-  out1[0] = x131;
-  out1[1] = x124;
-  out1[2] = x126;
-  out1[3] = x128;
-}
-
-with input bounds (Some [Some [0x0 ~> 0xffffffffffffffff], Some [0x0 ~> 0xffffffffffffffff], Some [0x0 ~> 0xffffffffffffffff], Some [0x0 ~> 0xffffffffffffffff]], Some [Some [0x0 ~> 0xffffffffffffffff], Some [0x0 ~> 0xffffffffffffffff], Some [0x0 ~> 0xffffffffffffffff], Some [0x0 ~> 0xffffffffffffffff]]).
-"
-     : string
-Finished transaction in 8.123 secs (7.909u,0.142s) (successful)
-*)
 
   End compile.
 
